Move flushed points-to to separate file

src/examples/durable_stack.v
@@ -15,7 +15,7 @@ From self.base Require Import primitive_laws class_instances.
 From self.high Require Import proofmode wpc_proofmode or_lost.
 From self.high Require Import dprop abstract_state_instances modalities
      resources crash_weakestpre weakestpre weakestpre_na weakestpre_at
-     recovery_weakestpre lifted_modalities protocol no_buffer.
+     recovery_weakestpre lifted_modalities protocol no_buffer mapsto_na_flushed.
 From self.high.modalities Require Import fence.
 
 (* TODO: Add the necessary fences in this example. *)
@@ -80,89 +80,6 @@ Section constant_prot.
   Next Obligation. iIntros. by iApply post_crash_flush_pure. Qed.
 
 End constant_prot.
-
-Definition mapsto_na_flushed `{nvmFixedG Σ, nvmDeltaG Σ, AbstractState ST}
-           ℓ (prot : LocationProtocol ST) q (s : ST) : dProp Σ :=
-  ∃ (ss : list ST),
-    "%lastEq" ∷ ⌜ last ss = Some s ⌝ ∗
-    "pts" ∷ ℓ ↦_{prot}^{q} ss ∗
-    "#flushLb" ∷ flush_lb ℓ prot s.
-
-Section mapsto_na_flushed.
-  Context `{nvmFixedG Σ, nvmDeltaG Σ, AbstractState ST}.
-
-  Global Instance buffer_free_mapsto_na_flushed ℓ prot q (s : ST) :
-    BufferFree (mapsto_na_flushed ℓ prot q s).
-  Proof. apply _. Qed.
-
-  Lemma mapsto_na_flushed_agree ℓ prot q q' (s s' : ST) :
-    mapsto_na_flushed ℓ prot q s -∗ mapsto_na_flushed ℓ prot q' s' -∗ ⌜ s = s' ⌝.
-  Proof.
-    rewrite /mapsto_na_flushed.
-    iNamed 1.
-    iDestruct 1 as (ss' last') "[pts' lb']".
-    rewrite /mapsto_na. iNamed "pts".
-    simplify_eq.
-    iDestruct "pts'" as (??????) "(% & ? & ? & ? & %look & %nolater' & ? & ? & ? & ? & ? & ? & ? & ?)".
-    simplify_eq.
-    iDestruct (full_entry_unenc_agree with "hist [$]") as %<-.
-    iPureIntro.
-    apply (inj Some).
-    rewrite -lookupV -look.
-    f_equiv.
-    eapply map_no_later_Some_agree; try done.
-  Qed.
-
-  Lemma mapsto_na_flushed_split ℓ prot p q (s : ST) :
-    mapsto_na_flushed ℓ prot (p + q) s -∗
-    mapsto_na_flushed ℓ prot p s ∗ mapsto_na_flushed ℓ prot q s.
-  Proof.
-    iDestruct 1 as (ss last) "[[pts1 pts2] #flushLb]".
-    iSplitL "pts1"; iFrame "flushLb"; iExists ss; iFrame (last) "∗".
-  Qed.
-
-  Global Instance mapsto_na_flushed_fractional ℓ prot (s : ST) :
-    Fractional (λ q, mapsto_na_flushed ℓ prot q s).
-  Proof.
-    rewrite /Fractional.
-    intros p q.
-    iSplit.
-    - iApply mapsto_na_flushed_split.
-    - iIntros "[L R]".
-      iNamed "R".
-      iDestruct "L" as (??) "[[pts1' pts2'] _]".
-      (* This direction is more annoying to show (not impossible) *)
-  Abort.
-
-  (* Lemma mapsto_na_increasing_list ℓ p q (ss : list ST) : *)
-  (*   mapsto_na p ℓ q ss -∗ ⌜ increasing_list (⊑@{ST}) ss ⌝. *)
-  (* Proof. rewrite /mapsto_na. iNamed 1. iFrame (incrList). Qed. *)
-
-  Global Instance mapsto_na_flushed_post_crash_flushed ℓ prot q (s : ST) :
-    IntoCrashFlush (mapsto_na_flushed ℓ prot q s)
-                   (λ _, mapsto_na_flushed ℓ prot q s ∗ recovered_at ℓ s)%I.
-  Proof.
-    rewrite /IntoCrashFlush.
-    iNamed 1.
-    (* iDestruct 1 as (? ss eq) "[pts lb]". *)
-    iDestruct "flushLb" as "-#flushLb".
-    (* We could leave out these two lines, but [iCrashFlush] takes a looong time
-    to find the [IntoCrashFlush] instance. *)
-    (* iDestruct (mapsto_na_increasing_list with "pts") as %incr. *)
-    iDestruct (post_crash_mapsto_na with "pts") as "pts".
-    iDestruct (post_crash_flush_post_crash with "pts") as "pts".
-    iCrashFlush.
-    iDestruct "flushLb" as (s' ?) "(#r & ?)".
-    iDestruct (recovered_at_or_lost with "r pts") as "(%s'' & ? & pts & ?)".
-    iDestruct (recovered_at_agree with "r [$]") as %eq.
-    (* We can't prove that with this approach, but it is (will be) true. *)
-  Admitted.
-
-End mapsto_na_flushed.
-
-(* Global Instance mapsto_na_flushed_as_fractional `{nvmFixedG Σ, nvmDeltaG Σ, AbstractState ST} per l q v : *)
-(*   AsFractional (mapsto_na per l q v) (λ q, mapsto_na per l q v)%I q. *)
-(* Proof. split; [done | apply _]. Qed. *)
 
 Section definitions.
   Implicit Types (ℓ : loc).
