src/high/mapsto_na_flushed.v
@@ -1,0 +1,98 @@
+(* This in an implementation of a concurrent non-blocking stack.
+
+The stack is implemented as a linked list. *)
+
+From iris.bi Require Import lib.fractional.
+From iris.proofmode Require Import tactics.
+
+From self.high Require Import proofmode wpc_proofmode or_lost.
+From self.high Require Import dprop abstract_state_instances modalities
+     resources crash_weakestpre weakestpre weakestpre_na weakestpre_at
+     recovery_weakestpre protocol no_buffer.
+From self.high.modalities Require Import fence.
+
+Definition mapsto_na_flushed `{nvmFixedG Σ, nvmDeltaG Σ, AbstractState ST}
+           ℓ (prot : LocationProtocol ST) q (s : ST) : dProp Σ :=
+  ∃ (ss : list ST),
+    "%lastEq" ∷ ⌜ last ss = Some s ⌝ ∗
+    "pts" ∷ ℓ ↦_{prot}^{q} ss ∗
+    "#flushLb" ∷ flush_lb ℓ prot s.
+
+Section mapsto_na_flushed.
+  Context `{nvmFixedG Σ, nvmDeltaG Σ, AbstractState ST}.
+
+  Global Instance buffer_free_mapsto_na_flushed ℓ prot q (s : ST) :
+    BufferFree (mapsto_na_flushed ℓ prot q s).
+  Proof. apply _. Qed.
+
+  Lemma mapsto_na_flushed_agree ℓ prot q q' (s s' : ST) :
+    mapsto_na_flushed ℓ prot q s -∗ mapsto_na_flushed ℓ prot q' s' -∗ ⌜ s = s' ⌝.
+  Proof.
+    rewrite /mapsto_na_flushed.
+    iNamed 1.
+    iDestruct 1 as (ss' last') "[pts' lb']".
+    rewrite /mapsto_na. iNamed "pts".
+    simplify_eq.
+    iDestruct "pts'" as (??????) "(% & ? & ? & ? & %look & %nolater' & ? & ? & ? & ? & ? & ? & ? & ?)".
+    simplify_eq.
+    iDestruct (full_entry_unenc_agree with "hist [$]") as %<-.
+    iPureIntro.
+    apply (inj Some).
+    rewrite -lookupV -look.
+    f_equiv.
+    eapply map_no_later_Some_agree; try done.
+  Qed.
+
+  Lemma mapsto_na_flushed_split ℓ prot p q (s : ST) :
+    mapsto_na_flushed ℓ prot (p + q) s -∗
+    mapsto_na_flushed ℓ prot p s ∗ mapsto_na_flushed ℓ prot q s.
+  Proof.
+    iDestruct 1 as (ss last) "[[pts1 pts2] #flushLb]".
+    iSplitL "pts1"; iFrame "flushLb"; iExists ss; iFrame (last) "∗".
+  Qed.
+
+  Global Instance mapsto_na_flushed_fractional ℓ prot (s : ST) :
+    Fractional (λ q, mapsto_na_flushed ℓ prot q s).
+  Proof.
+    rewrite /Fractional.
+    intros p q.
+    iSplit.
+    - iApply mapsto_na_flushed_split.
+    - iIntros "[L R]".
+      iNamed "R".
+      iDestruct "L" as (??) "[[pts1' pts2'] _]".
+      (* This direction is more annoying to show (not impossible) *)
+  Abort.
+
+  (* Lemma mapsto_na_increasing_list ℓ p q (ss : list ST) : *)
+  (*   mapsto_na p ℓ q ss -∗ ⌜ increasing_list (⊑@{ST}) ss ⌝. *)
+  (* Proof. rewrite /mapsto_na. iNamed 1. iFrame (incrList). Qed. *)
+
+  Global Instance mapsto_na_flushed_post_crash_flushed ℓ prot q (s : ST) :
+    IntoCrashFlush
+      (mapsto_na_flushed ℓ prot q s)
+      (λ _, mapsto_na_flushed ℓ prot q (bumper prot s) ∗
+            recovered_at ℓ (bumper prot s))%I.
+  Proof.
+    rewrite /IntoCrashFlush.
+    iNamed 1.
+    (* iDestruct 1 as (? ss eq) "[pts lb]". *)
+    iDestruct "flushLb" as "-#flushLb".
+    (* We could leave out these two lines, but [iCrashFlush] takes a looong time
+    to find the [IntoCrashFlush] instance. *)
+    (* iDestruct (mapsto_na_increasing_list with "pts") as %incr. *)
+    iDestruct (post_crash_mapsto_na with "pts") as "pts".
+    iDestruct (post_crash_flush_post_crash with "pts") as "pts".
+    iCrashFlush.
+    iDestruct "flushLb" as (s' le) "(#rec & persistLb)".
+    iDestruct (recovered_at_or_lost with "rec pts") as "(%s'' & %in & pts & rec2)".
+    iDestruct (recovered_at_agree with "rec rec2") as %eq.
+    (* FIXME: We need to know that [s'] and [s''] are equal. *)
+    (* iExists ([_]). iFrame "pts flushLb". *)
+  Admitted.
+
+End mapsto_na_flushed.
+
+(* Global Instance mapsto_na_flushed_as_fractional `{nvmFixedG Σ, nvmDeltaG Σ, AbstractState ST} per l q v : *)
+(*   AsFractional (mapsto_na per l q v) (λ q, mapsto_na per l q v)%I q. *)
+(* Proof. split; [done | apply _]. Qed. *)
